wip: Linearlizability of the prototype; proved some cases

src/Prototype/Correctness.v
@@ -1,4 +1,4 @@
-Require Import List String Peano_dec Eqdep.
+Require Import Bool List String Peano_dec Eqdep.
 Require Import FnMap Language SingleValue.
 
 Ltac inv H := inversion H; subst; clear H.
@@ -10,7 +10,8 @@ Ltac dest_in :=
 Ltac dest_existT :=
   repeat match goal with
          | [H: existT _ _ _ = existT _ _ _ |- _] =>
-           (apply EqdepTheory.inj_pair2 in H; subst)
+           try (pose proof (eq_sigT_fst H); subst);
+           apply EqdepTheory.inj_pair2 in H; subst
          end.
 
 Section ParentSequential.
@@ -18,49 +19,96 @@ Section ParentSequential.
   Definition parentObj :=
     existT (fun st => Object SingleValueMsg st) ParentState parent :: nil.
 
+  Definition parentRequestFrom (os: ObjectState ParentState) :=
+    match ps_request_from (os_state os) with
+    | Some (from, _) => Some (from, parentIdx)
+    | None => None
+    end.
+
+  Ltac invert_step :=
+    repeat
+      match goal with
+      | [H: step _ _ _ _ _ _ _ |- _ ] => inv H
+      | [H: step_obj _ _ _ _ _ _ _ _ |- _ ] => inv H
+      end.
+
+  Ltac invert_step_rule :=
+    repeat
+      match goal with
+      | [H: step_rule _ _ _ = Some _ |- _] =>
+        simpl in H;
+        repeat
+          match goal with
+          | [H: match ?t with
+                | Some _ => Some _
+                | None => _
+                end = Some _ |- _] =>
+            let trs := fresh "trs" in
+            remember t as trs; destruct trs
+          end; try discriminate
+      | [H: Some _ = Some _ |- _] => inv H
+      end.
+
   Lemma parent_sequential':
     forall hst oss1 msgs1 oss2 msgs2,
       steps parentObj oss1 msgs1 hst oss2 msgs2 ->
-      forall pos ss,
-        find parentIdx oss1 = Some (existT _ (ParentState: Type) pos) ->
-        ss = match ps_request_from (os_state pos) with
-             | Some (from, _) => Some (from, parentIdx)
-             | None => None
-             end ->
-        Sequential' (intHistory (getIndices parentObj) hst) ss.
+      forall pos1 pos2,
+        find parentIdx oss1 = Some (existT _ (ParentState: Type) pos1) ->
+        find parentIdx oss2 = Some (existT _ (ParentState: Type) pos2) ->
+        Sequential' (intHistory (getIndices parentObj) hst)
+                    (parentRequestFrom pos1) (parentRequestFrom pos2).
   Proof.
-    induction 1; simpl; intros; auto; subst.
+    induction 1; simpl; intros; subst;
+      [rewrite H in H0; inv H0; dest_existT; reflexivity|].
 
-    inv H0; inv H6.
+    invert_step.
+
     - (* internal *)
-      inv H2; [|inv H6].
-      pose proof (eq_sigT_fst H6); subst; dest_existT.
+      dest_in; dest_existT.
+      cbv in H2; inv H2; dest_existT.
+      specialize (IHsteps _ _ H1 H6).
+      invert_step_rule.
 
-      specialize (IHsteps _ _ H1 eq_refl).
-
-      simpl in H3.
-      remember (ParentGetReq msg_in (os_state os)) as getReqV; destruct getReqV.
       + (* getReq *)
-        inv H3.
         destruct msg_in as [msg_in_type msg_in_from msg_in_to msg_in_content]; simpl in *.
-        unfold ParentGetReq in HeqgetReqV; simpl in HeqgetReqV.
+        unfold ParentGetReq in Heqtrs; simpl in Heqtrs.
         remember (from_external msg_in_from) as msg_in_from_ext.
         destruct msg_in_from_ext; try discriminate.
         destruct msg_in_content; try discriminate.
+        destruct msg_in_type; try discriminate.
         remember (os_state os) as oss.
         destruct oss as [oss_is_valid oss_value oss_request_from]; simpl in *.
         destruct oss_request_from; try discriminate.
-        destruct oss_is_valid; inv HeqgetReqV; simpl in *.
-        * admit.
-        * admit.
+        destruct oss_is_valid; inv Heqtrs; simpl in *.
+        * rewrite intHistory_app; simpl.
+          eapply sequential_app; eauto.
+          simpl; unfold parentRequestFrom; rewrite <-Heqoss; simpl.
+          split; auto.
+          unfold isObjectsMsg, buildMsg; simpl.
+          rewrite orb_true_r; simpl.
+          repeat split.
+        * rewrite intHistory_app; simpl.
+          eapply sequential_app; eauto.
+          simpl; unfold parentRequestFrom; rewrite <-Heqoss; simpl.
+          split; auto.
+          replace (isObjectsMsg
+                     (parentIdx :: nil)
+                     (buildMsg Req parentIdx (theOtherChild msg_in_from) SvmInvReq)) with false.
+          { reflexivity. }
+          { unfold isObjectsMsg, buildMsg.
+            unfold msg_to, msg_type.
+            apply eq_sym, orb_false_iff; split; auto.
+            destruct (in_dec _ _ _); auto.
+            simpl in i; destruct i; inv H4.
+            unfold theOtherChild in H9.
+            destruct (eq_nat_dec _ _) in H9; discriminate.
+          }
         
-      + remember (ParentSetReq msg_in (os_state os)) as setReqV; destruct setReqV.
-        * (* setReq *)
-          admit.
-        * remember (ParentInvResp msg_in (os_state os)) as invRespV;
-            destruct invRespV; [|discriminate].
-          (* invResp *)
-          admit.
+      + (* setReq *)
+        admit.
+
+      + (* invResp *)
+        admit.
 
     - (* external: contradiction *)
       exfalso; admit.
@@ -74,7 +122,11 @@ Section ParentSequential.
   Proof.
     unfold HistoryOf, Sequential; intros.
     destruct H as [oss [oims ?]].
-    eapply parent_sequential' in H; eauto; reflexivity.
+    pose proof H; apply steps_poststate_valid in H0.
+    - destruct H0; destruct H0 as [os ?].
+      eapply parent_sequential' in H; try reflexivity; eauto.
+    - repeat split.
+      eexists; reflexivity.
   Qed.
 
 End ParentSequential.
